WellFormed2.v
@@ -17,26 +17,31 @@ Require Import WellFormed.
 Module NatMapFacts := NatMapProperties.F.
 Module CacheletMapFacts := CacheletMapProperties.F.
 
+Definition disjoint_VPT (V: VPT): Prop :=
+  forall e ranV, NatMap.find e V = Some ranV ->
+  (forall e' ranV', e <> e' -> NatMap.find e' V = Some ranV' ->
+   (forall c, In c ranV -> ~In c ranV') /\ (forall c, In c ranV' -> ~In c ranV)).
+
 Definition wf3 (sigma: runtime_state): Prop :=
-  forall k mu rho pi lambda F V C R c e ranV,
+  forall k mu rho pi lambda F V C R e ranV,
   (sigma = runtime_state_value k mu rho pi) ->
   (NatMap.find lambda k = Some (single_level_cache F V C R)) ->
-  (V_range V e = Some ranV) ->
-  ((In c ranV -> ~In c F) /\ (In c F -> ~In c ranV)).
+  (NatMap.find e V = Some ranV) ->
+  ((forall c, In c ranV -> ~In c F) /\ (forall c, In c F -> ~In c ranV)) /\ NoDup(F) /\ NoDup(ranV) /\ disjoint_VPT(V).
 
 (* WF3 MLC Read *)
 Lemma wf3_mlc_read : forall lambda h_tree k e' m0 l0 D obs1 mu k' index psi psi'
-  F V C R F' V' C' R' c enc ranV ranV',
+  F V C R F' V' C' R' enc ranV ranV',
   well_defined_cache_tree h_tree ->
   mlc_read k e' m0 l0 lambda h_tree = mlc_read_valid D obs1 mu k' ->
   NatMap.find index k = Some psi ->
   NatMap.find index k' = Some psi' ->
   psi = single_level_cache F V C R ->
   psi' = single_level_cache F' V' C' R' ->
-  V_range V enc = Some ranV ->
-  V_range V' enc = Some ranV' ->
-  ((In c ranV -> ~In c F) /\ (In c F -> ~In c ranV)) ->
-  ((In c ranV' -> ~In c F') /\ (In c F' -> ~In c ranV')).
+  NatMap.find enc V = Some ranV ->
+  NatMap.find enc V' = Some ranV' ->
+  ((forall c, In c ranV -> ~In c F) /\ (forall c, In c F -> ~In c ranV)) /\ NoDup(F) /\ NoDup(ranV) /\ disjoint_VPT(V) ->
+  ((forall c, In c ranV' -> ~In c F') /\ (forall c, In c F' -> ~In c ranV')) /\ NoDup(F') /\ NoDup(ranV') /\ disjoint_VPT(V').
 Proof.
   unfold mlc_read.
   intros lambda h_tree.
@@ -69,17 +74,17 @@ Proof.
     injection H0; injection A0; injection A1; intros; subst; clear A0 A1.
     assert (H10 := H9).
     destruct s; destruct s1.
-    apply (cc_hit_read_f (single_level_cache c1 v w s) e' l0 D obs1 c0
-    (single_level_cache c2 v0 w0 s0) c1 v w s c2 v0 w0 s0) in H9.
-    apply (cc_hit_read_v (single_level_cache c1 v w s) e' l0 D obs1 c0
-    (single_level_cache c2 v0 w0 s0) c1 v w s c2 v0 w0 s0) in H10.
+    apply (cc_hit_read_f (single_level_cache c0 v w s) e' l0 D obs1 c
+    (single_level_cache c1 v0 w0 s0) c0 v w s c1 v0 w0 s0) in H9.
+    apply (cc_hit_read_v (single_level_cache c0 v w s) e' l0 D obs1 c
+    (single_level_cache c1 v0 w0 s0) c0 v w s c1 v0 w0 s0) in H10.
     subst.
     {
       case_eq (eqb a index).
       {
         intros. apply cmp_to_eq in H3. subst.
         rewrite -> H1 in H8.
-        injection H8; intros; subst c2 v0 w s.
+        injection H8; intros; subst c1 v0 w s.
         assert (NatMap.find index (NatMap.add index (single_level_cache F V w0 s0) k) =
         Some (single_level_cache F V w0 s0)).
         apply NatMapFacts.add_eq_o. reflexivity.
@@ -90,7 +95,7 @@ Proof.
       }
       {
         intros. apply cmp_to_uneq in H3.
-        assert (NatMap.find index (NatMap.add a (single_level_cache c2 v0 w0 s0) k) = NatMap.find index k).
+        assert (NatMap.find index (NatMap.add a (single_level_cache c1 v0 w0 s0) k) = NatMap.find index k).
         apply NatMapFacts.add_neq_o. exact H3.
         rewrite -> H2 in H4.
         rewrite -> H1 in H4.
@@ -118,13 +123,13 @@ Proof.
         destruct s.
         assert (H12 := H11).
         destruct s1.
-        apply (cc_update_f (single_level_cache c1 v w s) e' D l0 c0 (single_level_cache c2 v0 w0 s0)
-        c1 v w s c2 v0 w0 s0) in H11.
-        apply (cc_update_v (single_level_cache c1 v w s) e' D l0 c0 (single_level_cache c2 v0 w0 s0)
-        c1 v w s c2 v0 w0 s0) in H12.
+        apply (cc_update_f (single_level_cache c0 v w s) e' D l0 c (single_level_cache c1 v0 w0 s0)
+        c0 v w s c1 v0 w0 s0) in H11.
+        apply (cc_update_v (single_level_cache c0 v w s) e' D l0 c (single_level_cache c1 v0 w0 s0)
+        c0 v w s c1 v0 w0 s0) in H12.
         subst.
-        assert (NatMap.find index (NatMap.add index (single_level_cache c2 v0 w0 s0) m) =
-        Some (single_level_cache c2 v0 w0 s0)).
+        assert (NatMap.find index (NatMap.add index (single_level_cache c1 v0 w0 s0) m) =
+        Some (single_level_cache c1 v0 w0 s0)).
         apply NatMapFacts.add_eq_o. reflexivity.
         rewrite -> H3 in H2.
         rewrite -> H8 in H1.
@@ -144,7 +149,7 @@ Proof.
         destruct l.
         {
           apply (IHl root_node WFH1 k e' m0 l0 D obs1 o m index (single_level_cache F V C R)
-          (single_level_cache F' V' C' R') F V C R F' V' C' R' c enc ranV ranV').
+          (single_level_cache F' V' C' R') F V C R F' V' C' R' enc ranV ranV').
           exact WFH.
           unfold mlc_write. exact H10.
           exact H1.
@@ -160,13 +165,13 @@ Proof.
         {
           destruct lambda.
           rewrite -> WFH1 in IHTREE. discriminate.
-          specialize (WFH3 c1 a (p :: l) IHTREE).
+          specialize (WFH3 c0 a (p :: l) IHTREE).
           unfold get_cache_ID_path in IHTREE. discriminate.
           specialize (WFH2 p0 a (p :: l) IHTREE).
           injection WFH2; intros; subst.
           apply (H p0 p l) in IHTREE.
           apply (IHl (cache_node p) IHTREE k e' m0 l0 D obs1 o m index (single_level_cache F V C R)
-          (single_level_cache F' V' C' R') F V C R F' V' C' R' c enc ranV ranV').
+          (single_level_cache F' V' C' R') F V C R F' V' C' R' enc ranV ranV').
           exact WFH.
           unfold mlc_write. exact H10.
           exact H1.
@@ -203,17 +208,17 @@ Qed.
 
 (* WF3 MLC Write *)
 Lemma wf3_mlc_write : forall lambda h_tree k e' m0 l0 v D obs1 mu k' index psi psi'
-  F V C R F' V' C' R' c enc ranV ranV',
+  F V C R F' V' C' R' enc ranV ranV',
   well_defined_cache_tree h_tree ->
   mlc_write k e' m0 l0 v lambda h_tree = mlc_write_valid D obs1 mu k' ->
   NatMap.find index k = Some psi ->
   NatMap.find index k' = Some psi' ->
   psi = single_level_cache F V C R ->
   psi' = single_level_cache F' V' C' R' ->
-  V_range V enc = Some ranV ->
-  V_range V' enc = Some ranV' ->
-  ((In c ranV -> ~In c F) /\ (In c F -> ~In c ranV)) ->
-  ((In c ranV' -> ~In c F') /\ (In c F' -> ~In c ranV')).
+  NatMap.find enc V = Some ranV ->
+  NatMap.find enc V' = Some ranV' ->
+  ((forall c, In c ranV -> ~In c F) /\ (forall c, In c F -> ~In c ranV)) /\ NoDup(F) /\ NoDup(ranV) /\ disjoint_VPT(V) ->
+  ((forall c, In c ranV' -> ~In c F') /\ (forall c, In c F' -> ~In c ranV')) /\ NoDup(F') /\ NoDup(ranV') /\ disjoint_VPT(V').
 Proof.
   unfold mlc_write.
   intros lambda h_tree.
@@ -223,7 +228,7 @@ Proof.
   induction l.
   {
     intros lambda IHTREE k e' m0 l0 v D obs1 mu k' index psi psi'
-    F V C R F' V' C' R' c enc ranV ranV' WFH1; intros.
+    F V C R F' V' C' R' enc ranV ranV' WFH1; intros.
     destruct (get_cache_ID_path lambda h_tree).
     injection IHTREE; intros; subst.
     unfold recursive_mlc_write in H.
@@ -241,7 +246,7 @@ Proof.
   }
   {
     intros lambda IHTREE k e' m0 l0 v D obs1 mu k' index psi psi'
-    F V C R F' V' C' R' c enc ranV ranV' WFH1; intros.
+    F V C R F' V' C' R' enc ranV ranV' WFH1; intros.
     unfold recursive_mlc_write in H.
     fold recursive_mlc_write in H.
     case_eq (NatMap.find a k). intros.
@@ -251,17 +256,17 @@ Proof.
     injection H; injection A0; injection A1; intros; subst; clear A0 A1.
     assert (H9 := H8).
     destruct s; destruct s1.
-    apply (cc_hit_write_f (single_level_cache c1 v0 w s) e' (address b d1) v D c0
-    (single_level_cache c2 v1 w0 s0) c1 v0 w s c2 v1 w0 s0) in H8.
-    apply (cc_hit_write_v (single_level_cache c1 v0 w s) e' (address b d1) v D c0
-    (single_level_cache c2 v1 w0 s0) c1 v0 w s c2 v1 w0 s0) in H9.
+    apply (cc_hit_write_f (single_level_cache c0 v0 w s) e' (address b d1) v D c
+    (single_level_cache c1 v1 w0 s0) c0 v0 w s c1 v1 w0 s0) in H8.
+    apply (cc_hit_write_v (single_level_cache c0 v0 w s) e' (address b d1) v D c
+    (single_level_cache c1 v1 w0 s0) c0 v0 w s c1 v1 w0 s0) in H9.
     subst.
     {
       case_eq (eqb a index).
       {
         intros. apply cmp_to_eq in H2. subst.
         rewrite -> H0 in H7.
-        injection H7; intros; subst c2 v1 w s.
+        injection H7; intros; subst c1 v1 w s.
         assert (NatMap.find index (NatMap.add index (single_level_cache F V w0 s0) k) =
         Some (single_level_cache F V w0 s0)).
         apply NatMapFacts.add_eq_o. reflexivity.
@@ -272,7 +277,7 @@ Proof.
       }
       {
         intros. apply cmp_to_uneq in H2.
-        assert (NatMap.find index (NatMap.add a (single_level_cache c2 v1 w0 s0) k) = NatMap.find index k).
+        assert (NatMap.find index (NatMap.add a (single_level_cache c1 v1 w0 s0) k) = NatMap.find index k).
         apply NatMapFacts.add_neq_o. exact H2.
         rewrite -> H1 in H3.
         rewrite -> H0 in H3.
@@ -300,13 +305,13 @@ Proof.
         destruct s.
         assert (H11 := H10).
         destruct s1.
-        apply (cc_update_f (single_level_cache c1 v0 w s) e' D l0 c0 (single_level_cache c2 v1 w0 s0)
-        c1 v0 w s c2 v1 w0 s0) in H10.
-        apply (cc_update_v (single_level_cache c1 v0 w s) e' D l0 c0 (single_level_cache c2 v1 w0 s0)
-        c1 v0 w s c2 v1 w0 s0) in H11.
+        apply (cc_update_f (single_level_cache c0 v0 w s) e' D l0 c (single_level_cache c1 v1 w0 s0)
+        c0 v0 w s c1 v1 w0 s0) in H10.
+        apply (cc_update_v (single_level_cache c0 v0 w s) e' D l0 c (single_level_cache c1 v1 w0 s0)
+        c0 v0 w s c1 v1 w0 s0) in H11.
         subst.
-        assert (NatMap.find index (NatMap.add index (single_level_cache c2 v1 w0 s0) m1) =
-        Some (single_level_cache c2 v1 w0 s0)).
+        assert (NatMap.find index (NatMap.add index (single_level_cache c1 v1 w0 s0) m1) =
+        Some (single_level_cache c1 v1 w0 s0)).
         apply NatMapFacts.add_eq_o. reflexivity.
         rewrite -> H2 in H1.
         rewrite -> H7 in H0.
@@ -326,7 +331,7 @@ Proof.
         destruct l.
         {
           apply (IHl root_node WFH1 k e' m0 l0 v D o mu m1 index (single_level_cache F V C R)
-          (single_level_cache F' V' C' R') F V C R F' V' C' R' c enc ranV ranV').
+          (single_level_cache F' V' C' R') F V C R F' V' C' R' enc ranV ranV').
           exact WFH.
           unfold mlc_write. exact H9.
           exact H0.
@@ -342,13 +347,13 @@ Proof.
         {
           destruct lambda.
           rewrite -> WFH1 in IHTREE. discriminate.
-          specialize (WFH3 c1 a (p :: l) IHTREE).
+          specialize (WFH3 c0 a (p :: l) IHTREE).
           unfold get_cache_ID_path in IHTREE. discriminate.
           specialize (WFH2 p0 a (p :: l) IHTREE).
           injection WFH2; intros; subst.
           apply (WFH4 p0 p l) in IHTREE.
           apply (IHl (cache_node p) IHTREE k e' m0 l0 v D o mu m1 index (single_level_cache F V C R)
-          (single_level_cache F' V' C' R') F V C R F' V' C' R' c enc ranV ranV').
+          (single_level_cache F' V' C' R') F V C R F' V' C' R' enc ranV ranV').
           exact WFH.
           unfold mlc_write. exact H9.
           exact H0.
@@ -382,163 +387,373 @@ Proof.
 Qed.
 
 (* WF3 MLC Deallocation *)
-Lemma V_range_add_empty : forall V r enc ranV ranV' c,
-  V_range V enc = Some ranV ->
-  V_range (NatMap.add r (NatMap.empty way_mask) V) enc = Some ranV' ->
-  In c ranV' -> In c ranV.
+Lemma wf3_clear_remapping_list : forall r ranV F V C R F' V' C' R' ranV',
+  clear_remapping_list r ranV F V C R = Some (single_level_cache F' V' C' R') ->
+  NatMap.find r V = Some ranV ->
+  NatMap.find r V' = Some ranV' ->
+  ((forall c, In c ranV -> ~ In c F) /\ (forall c, In c F -> ~ In c ranV)) /\ NoDup(F) /\ NoDup(ranV) /\ disjoint_VPT(V)  ->
+  ((forall c, In c ranV' -> ~ In c F') /\ (forall c, In c F' -> ~ In c ranV')) /\ NoDup(F') /\ NoDup(ranV') /\ disjoint_VPT(V') .
 Proof.
-  intros.
-  unfold V_range in *.
-  case_eq (NatMap.find enc V). intros.
-  assert (A0 := H2). destruct (NatMap.find enc V) in H, A0.
-  case_eq (NatMap.find (elt:=remapping_list) enc (NatMap.add r (NatMap.empty way_mask) V)). intros.
-  assert (A1 := H3). destruct (NatMap.find (elt:=remapping_list) enc (NatMap.add r (NatMap.empty way_mask) V)) in H0, A1.
-  injection A0; injection A1; intros; subst r3 r0; clear A0 A1.
-  case_eq (eqb r enc); intros.
-  apply cmp_to_eq in H4; subst r.
-  assert (NatMap.find (elt:=remapping_list) enc (NatMap.add enc (NatMap.empty way_mask) V) = Some (NatMap.empty way_mask)).
-  apply NatMapFacts.add_eq_o. reflexivity.
-  rewrite -> H3 in H4.
-  injection H4; intros; subst.
-  injection H0; intros; subst.
-  unfold In in H1. destruct H1.
-  apply cmp_to_uneq in H4.
-  assert (NatMap.find (elt:=remapping_list) enc (NatMap.add r (NatMap.empty way_mask) V)
-  = NatMap.find (elt:=remapping_list) enc V).
-  apply NatMapFacts.add_neq_o. exact H4.
-  rewrite -> H2 in H5.
-  rewrite -> H3 in H5.
-  injection H5; intros; subst r2.
-  rewrite -> H0 in H.
-  injection H; intros; subst ranV'.
-  exact H1.
-  discriminate.
-  intros; destruct (NatMap.find (elt:=remapping_list) enc (NatMap.add r (NatMap.empty way_mask) V)).
-  discriminate.
-  discriminate.
-  discriminate.
-  intros; destruct (NatMap.find enc V).
-  discriminate.
-  discriminate.
+  intros r l.
+  induction l.
+  {
+    intros.
+    unfold clear_remapping_list in H.
+    injection H; intros; subst.
+    assert (NatMap.find r (NatMap.remove r V) = None).
+    apply NatMapFacts.remove_eq_o; reflexivity.
+    rewrite -> H3 in H1. discriminate.
+  }
+  {
+    intros.
+    unfold clear_remapping_list in H.
+    fold clear_remapping_list in H.
+    destruct a.
+    case_eq (NatMap.find s R). intros.
+    assert (A0 := H3). destruct (NatMap.find s R) in A0, H.
+    case_eq (cachelet_invalidation C (w, s)). intros.
+    assert (A1 := H4). destruct (cachelet_invalidation C (w, s)) in A1, H.
+    injection A0; injection A1; intros; subst w1 p; clear A0 A1.
+    apply (IHl ((w, s) :: F) (NatMap.add r l V) w0 (NatMap.add s (update p0 w
+    (enclave_ID_active r)) R) F' V' C' R' ranV').
+    exact H.
+    apply NatMapFacts.add_eq_o; reflexivity.
+    exact H1.
+    {
+      destruct H2; destruct H2; destruct H5; destruct H7.
+      split; split.
+      intros. intros contra.
+      apply in_inv in contra. destruct contra.
+      subst c.
+      apply NoDup_cons_iff in H7. destruct H7.
+      apply H7 in H9. exact H9.
+      apply H6 in H10.
+      assert (In c ((w, s) :: l)).
+      apply in_cons; exact H9.
+      apply H10 in H11. exact H11.
+      intros. intros contra.
+      apply in_inv in H9. destruct H9.
+      subst c.
+      apply NoDup_cons_iff in H7. destruct H7.
+      apply H7 in contra. exact contra.
+      apply H6 in H9.
+      assert (In c ((w, s) :: l)).
+      apply in_cons; exact contra.
+      apply H9 in H10. exact H10.
+      constructor.
+      apply NoDup_cons_iff in H7. destruct H7.
+      intros contra.
+      apply H6 in contra.
+      unfold not in contra.
+      assert (In (w, s) ((w, s) :: l)).
+      apply in_eq; reflexivity.
+      apply contra in H10. exact H10.
+      exact H5. split.
+      apply NoDup_cons_iff in H7. destruct H7. exact H9.
+      {
+        unfold disjoint_VPT in *.
+        intros e ranV H9 e' ranV'0 H10 H11.
+        case_eq (eqb e r); case_eq (eqb e' r); intros.
+        apply cmp_to_eq in H12, H13; subst.
+        unfold not in H10; destruct H10; reflexivity.
+        apply cmp_to_uneq in H12; apply cmp_to_eq in H13; subst.
+        assert (NatMap.find (elt:=remapping_list) r (NatMap.add r l V) = Some l).
+        apply NatMapFacts.add_eq_o; reflexivity.
+        rewrite -> H9 in H13; injection H13; intros; subst.
+        assert (NatMap.find (elt:=remapping_list) e' (NatMap.add r l V) = NatMap.find e' V).
+        apply NatMapFacts.add_neq_o; exact H10.
+        rewrite -> H11 in H14; apply eq_sym in H14.
+        specialize (H8 r ((w, s) :: l) H0 e' ranV'0 H10 H14); destruct H8.
+        split; intros.
+        intros contra. apply H15 in contra.
+        apply (in_cons (w, s) c l) in H16.
+        apply contra in H16. destruct H16.
+        intros contra. apply (in_cons (w, s) c l) in contra.
+        apply H8 in contra. apply contra in H16. destruct H16.
+        apply cmp_to_eq in H12; apply cmp_to_uneq in H13; subst.
+        assert (NatMap.find (elt:=remapping_list) e (NatMap.add r l V) = NatMap.find e V).
+        apply NatMapFacts.add_neq_o; apply not_eq_sym; exact H10.
+        rewrite -> H9 in H12; apply eq_sym in H12.
+        assert (NatMap.find (elt:=remapping_list) r (NatMap.add r l V) = Some l).
+        apply NatMapFacts.add_eq_o; reflexivity.
+        rewrite -> H11 in H14; injection H14; intros; subst.
+        specialize (H8 e ranV H12 r ((w, s) :: l) H10 H0); destruct H8.
+        split; intros.
+        intros contra. apply (in_cons (w, s) c l) in contra.
+        apply H15 in contra. apply contra in H16. destruct H16.
+        intros contra. apply H8 in contra.
+        apply (in_cons (w, s) c l) in H16.
+        apply contra in H16. destruct H16.
+        apply cmp_to_uneq in H12, H13.
+        assert (NatMap.find (elt:=remapping_list) e (NatMap.add r l V) = NatMap.find e V).
+        apply NatMapFacts.add_neq_o; apply not_eq_sym; exact H13.
+        assert (NatMap.find (elt:=remapping_list) e' (NatMap.add r l V) = NatMap.find e' V).
+        apply NatMapFacts.add_neq_o; apply not_eq_sym; exact H12.
+        rewrite -> H9 in H14. rewrite -> H11 in H15. apply eq_sym in H14, H15.
+        specialize (H8 e ranV H14 e' ranV'0 H10 H15); exact H8.
+      }
+    }
+    discriminate.
+    intros; destruct (cachelet_invalidation C (w, s)).
+    discriminate.
+    discriminate.
+    discriminate.
+    intros; destruct (NatMap.find s R).
+    discriminate.
+    discriminate.
+  }
 Qed.
 
-Lemma wf3_free_cachelets : forall w0 r k F V C R F' V' C' R' r0 c enc ranV ranV',
-  ((In c ranV -> ~In c F) /\ (In c F -> ~In c ranV)) ->
-  V_range V enc = Some ranV ->
-  V_range V' enc = Some ranV' ->
-  NatMap.find r V = Some r0 ->
-  free_cachelets r k w0 F V C R = Some (single_level_cache F' V' C' R') ->
-  ((In c ranV' -> ~In c F') /\ (In c F' -> ~In c ranV')).
+Lemma clear_remapping_list_ranV : forall r l F V C R F' V' C' R' e ranV ranV',
+  r <> e -> clear_remapping_list r l F V C R = Some (single_level_cache F' V' C' R') ->
+  NatMap.find e V = Some ranV ->
+  NatMap.find e V' = Some ranV' ->
+  ranV = ranV'.
 Proof.
-  intros w0.
-  induction w0.
+  intros r l.
+  induction l.
   {
     intros.
-    unfold free_cachelets in H3.
+    unfold clear_remapping_list in H0.
+    injection H0; intros; subst.
+    assert (NatMap.find e (NatMap.remove r V) = NatMap.find e V).
+    apply NatMapFacts.remove_neq_o; exact H.
+    rewrite -> H1 in H3; rewrite -> H2 in H3;
     injection H3; intros; subst.
-    rewrite -> H0 in H1.
-    injection H1; intros; subst.
-    exact H.
+    reflexivity.
   }
   {
     intros.
-    unfold free_cachelets in H3.
-    fold free_cachelets in H3.
-    case_eq (NatMap.find k R). intros.
-    assert (A0 := H4). destruct (NatMap.find k R) in A0, H3.
-    case_eq (cachelet_invalidation C (a, k)). intros.
-    assert (A1 := H5). destruct (cachelet_invalidation C (a, k)) in A1, H3.
-    injection A0; injection A1; intros; subst p0 w1; clear A0 A1.
-    apply (IHw0 r k ((a, k) :: F) V w (NatMap.add k (update p a (enclave_ID_active r)) R)
-    F' V' C' R' r0 c enc ranV ranV').
-    destruct H.
-    split.
-    {
-      intros.
-      intros contra.
-      apply in_inv in contra.
-      destruct contra.
-      give_up.
-      apply H6 in H8.
-      apply H8 in H7.
-      exact H7.
-    }
-    give_up.
-    give_up.
-    give_up.
-    give_up.
-    give_up.
-    give_up.
-    give_up.
-    give_up.
-    give_up.
-  }
-Admitted.
-
-Lemma wf3_clear_remapping_list : forall r r1 F V C R F' V' C' R' c enc ranV ranV',
-  ((In c ranV -> ~In c F) /\ (In c F -> ~In c ranV)) ->
-  V_range V enc = Some ranV ->
-  V_range V' enc = Some ranV' ->
-  NatMap.In r V ->
-  clear_remapping_list r (NatMapProperties.to_list r1) F V C R = Some (single_level_cache F' V' C' R') ->
-  ((In c ranV' -> ~In c F') /\ (In c F' -> ~In c ranV')).
-Proof.
-  intros r r0.
-  induction (NatMapProperties.to_list r0).
-  {
-    intros.
-    assert (H4 := H3).
-    apply (clear_remapping_list_v r (NatMap.empty way_mask) F V C R F' V' C' R' enc) in H4.
-    unfold clear_remapping_list in H3.
-    injection H3; intros; subst F' V' C' R'.
-    assert (In c ranV' -> In c ranV).
-    apply (V_range_add_empty V r enc ranV ranV' c).
-    exact H0. exact H1.
-    destruct H.
-    split.
-    {
-      intros.
-      apply H.
-      apply H5.
-      exact H7.
-    }
-    {
-      intros.
-      intros contra.
-      apply H5 in contra.
-      apply H in contra.
-      apply contra in H7.
-      destruct H7.
-    }
-    exact H2.
-  }
-  {
-    intros.
-    unfold clear_remapping_list in H3.
-    fold clear_remapping_list in H3.
+    unfold clear_remapping_list in H0.
+    fold clear_remapping_list in H0.
     destruct a.
-    case_eq (free_cachelets r k w F V C R). intros.
-    assert (A0 := H4). destruct (free_cachelets r k w F V C R) in A0, H3.
-    destruct s; destruct s0.
-    injection A0; intros; subst; clear A0.
-    give_up.
-    give_up.
-    give_up.
+    destruct (NatMap.find s R). destruct (cachelet_invalidation C (w, s)).
+    apply (IHl ((w, s) :: F) (NatMap.add r l V) w0 (NatMap.add s (update p w
+    (enclave_ID_active r)) R) F' V' C' R' e ranV ranV').
+    exact H. exact H0.
+    rewrite <- H1.
+    apply NatMapFacts.add_neq_o; exact H.
+    exact H2.
+    discriminate.
+    discriminate.
   }
-Admitted.
+Qed.
 
+Lemma disjoint_VPT_remove : forall r V,
+  disjoint_VPT V -> disjoint_VPT (NatMap.remove r V).
+Proof.
+  intros.
+  unfold disjoint_VPT in *; intros.
+  assert (NatMap.find (elt:=remapping_list) r (NatMap.remove r V) = None).
+  apply NatMapFacts.remove_eq_o; reflexivity.
+  case_eq (eqb e r); intros.
+  apply cmp_to_eq in H4; subst.
+  rewrite -> H0 in H3; discriminate.
+  case_eq (eqb e' r); intros.
+  apply cmp_to_eq in H5; subst.
+  rewrite -> H2 in H3; discriminate.
+  apply cmp_to_uneq in H4, H5.
+  assert (NatMap.find (elt:=remapping_list) e (NatMap.remove r V) = NatMap.find e V).
+  apply NatMapFacts.remove_neq_o; apply not_eq_sym; exact H4.
+  assert (NatMap.find (elt:=remapping_list) e' (NatMap.remove r V) = NatMap.find e' V).
+  apply NatMapFacts.remove_neq_o; apply not_eq_sym; exact H5.
+  rewrite -> H0 in H6; rewrite -> H2 in H7; apply eq_sym in H6, H7.
+  specialize (H e ranV H6 e' ranV' H1 H7).
+  exact H.
+Qed.
 
-Lemma wf3_mlc_dealloc : forall lambda h_tree state k k' index psi psi' F V C R F' V' C' R' c enc ranV ranV',
+Lemma disjoint_VPT_add : forall r V q l,
+  NatMap.find r V = Some (q :: l) ->
+  disjoint_VPT V -> disjoint_VPT (NatMap.add r l V).
+Proof.
+  intros.
+  unfold disjoint_VPT in *; intros.
+  case_eq (eqb e r); case_eq (eqb e' r); intros.
+  apply cmp_to_eq in H4, H5; subst.
+  unfold not in H2; destruct H2; reflexivity.
+  apply cmp_to_uneq in H4; apply cmp_to_eq in H5; subst.
+  assert (NatMap.find (elt:=remapping_list) r (NatMap.add r l V) = Some l).
+  apply NatMapFacts.add_eq_o; reflexivity.
+  assert (NatMap.find (elt:=remapping_list) e' (NatMap.add r l V)
+  = NatMap.find (elt:=remapping_list) e' V).
+  apply NatMapFacts.add_neq_o; exact H2.
+  rewrite -> H1 in H5; injection H5; intros; subst.
+  rewrite -> H3 in H6; apply eq_sym in H6.
+  specialize (H0 r (q :: l) H e' ranV' H2 H6); destruct H0.
+  split; intros.
+  apply (in_cons q c l) in H8. apply H0 in H8. exact H8.
+  apply H7 in H8. intros contra. apply (in_cons q c l) in contra.
+  apply H8 in contra. exact contra.
+  apply cmp_to_uneq in H5; apply cmp_to_eq in H4; subst.
+  assert (NatMap.find (elt:=remapping_list) r (NatMap.add r l V) = Some l).
+  apply NatMapFacts.add_eq_o; reflexivity.
+  assert (NatMap.find (elt:=remapping_list) e (NatMap.add r l V)
+  = NatMap.find (elt:=remapping_list) e V).
+  apply NatMapFacts.add_neq_o; apply not_eq_sym; exact H2.
+  rewrite -> H3 in H4; injection H4; intros; subst.
+  rewrite -> H1 in H6; apply eq_sym in H6.
+  specialize (H0 e ranV H6 r (q :: l) H2 H); destruct H0.
+  split; intros.
+  apply H0 in H8. intros contra. apply (in_cons q c l) in contra.
+  apply H8 in contra. exact contra.
+  apply (in_cons q c l) in H8. apply H7 in H8. exact H8.
+  apply cmp_to_uneq in H4, H5.
+  assert (NatMap.find (elt:=remapping_list) e (NatMap.add r l V)
+  = NatMap.find (elt:=remapping_list) e V).
+  apply NatMapFacts.add_neq_o; apply not_eq_sym; exact H5.
+  assert (NatMap.find (elt:=remapping_list) e' (NatMap.add r l V)
+  = NatMap.find (elt:=remapping_list) e' V).
+  apply NatMapFacts.add_neq_o; apply not_eq_sym; exact H4.
+  rewrite -> H1 in H6; rewrite -> H3 in H7; apply eq_sym in H6, H7.
+  apply (H0 e ranV H6 e' ranV' H2 H7).
+Qed.
+
+Lemma wf3_clear_remapping_list_uneq : forall r l F V C R F' V' C' R' e ranV ranV',
+  e <> r -> clear_remapping_list r l F V C R = Some (single_level_cache F' V' C' R') ->
+  NatMap.find r V = Some l ->
+  NatMap.find e V = Some ranV ->
+  NatMap.find e V' = Some ranV' ->
+  ((forall c, In c ranV -> ~ In c F) /\ (forall c, In c F -> ~ In c ranV)) /\ NoDup(F) /\ NoDup(ranV) /\ disjoint_VPT(V) ->
+  ((forall c, In c l -> ~ In c F) /\ (forall c, In c F -> ~ In c l)) /\ NoDup(l) ->
+  ((forall c, In c ranV' -> ~ In c F') /\ (forall c, In c F' -> ~ In c ranV')) /\ NoDup(F') /\ NoDup(ranV') /\ disjoint_VPT(V').
+Proof.
+  intros r l.
+  induction l.
+  {
+    intros.
+    unfold clear_remapping_list in H0.
+    injection H0; intros; subst.
+    assert (NatMap.find e (NatMap.remove r V) = NatMap.find e V).
+    apply NatMapFacts.remove_neq_o; apply not_eq_sym; exact H.
+    rewrite -> H3 in H6; rewrite -> H2 in H6.
+    injection H6; intros; subst.
+    split; destruct H4. exact H4.
+    split; destruct H7. exact H7.
+    split; destruct H8. exact H8.
+    apply disjoint_VPT_remove; exact H9.
+  }
+  {
+    intros.
+    unfold clear_remapping_list in H0.
+    fold clear_remapping_list in H0.
+    destruct a.
+    case_eq (NatMap.find s R). intros.
+    assert (A0 := H6). destruct (NatMap.find s R) in A0, H0.
+    case_eq (cachelet_invalidation C (w, s)). intros.
+    assert (A1 := H7). destruct (cachelet_invalidation C (w, s)) in A1, H0.
+    injection A0; injection A1; intros; subst w1 p; clear A0 A1.
+    assert (ranV = ranV').
+    apply (clear_remapping_list_ranV r l ((w, s) :: F) (NatMap.add r l V) w0 (NatMap.add s
+    (update p0 w (enclave_ID_active r)) R) F' V' C' R' e ranV ranV').
+    apply not_eq_sym; exact H. exact H0.
+    rewrite <- H2. apply NatMapFacts.add_neq_o. apply not_eq_sym; exact H.
+    exact H3. subst ranV'.
+    apply (IHl ((w, s) :: F) (NatMap.add r l V) w0 (NatMap.add s (update p0 w
+    (enclave_ID_active r)) R) F' V' C' R' e ranV ranV).
+    exact H. exact H0.
+    apply NatMapFacts.add_eq_o; reflexivity.
+    rewrite <- H2. apply NatMapFacts.add_neq_o; apply not_eq_sym; exact H.
+    exact H3.
+    {
+      destruct H4; destruct H4; destruct H8; destruct H10.
+      destruct H5 as [ H5 N ]. destruct H5 as [ H5 H5' ].
+      assert (V0 := H11).
+      unfold disjoint_VPT in H11.
+      specialize (H11 e ranV H2 r ((w, s) :: l) H H1); destruct H11.
+      split; split.
+      intros. intros contra.
+      apply in_inv in contra. destruct contra.
+      subst c. apply H11 in H13.
+      unfold In in H13. destruct H13. left; reflexivity.
+      apply H9 in H14. apply H14 in H13. exact H13.
+      intros. intros contra.
+      apply in_inv in H13. destruct H13.
+      subst c. apply H11 in contra.
+      unfold In in contra. destruct contra. left; reflexivity.
+      apply H9 in H13. apply H13 in contra. exact contra.
+      constructor.
+      assert (In (w, s) ((w, s) :: l)).
+      apply in_eq; reflexivity.
+      apply H5 in H13. exact H13. exact H8.
+      split. exact H10.
+      apply (disjoint_VPT_add r V (w, s) l).
+      exact H1. exact V0.
+    }
+    destruct H5; destruct H5.
+    split. split; intros.
+    intros contra. apply in_inv in contra. destruct contra. subst c.
+    apply NoDup_cons_iff in H8. destruct H8.
+    apply H8 in H10. exact H10.
+    apply (in_cons (w, s) c l) in H10. apply H9 in H11.
+    apply H11 in H10. exact H10.
+    intros contra. apply in_inv in H10. destruct H10. subst c.
+    apply NoDup_cons_iff in H8. destruct H8.
+    apply H8 in contra. exact contra.
+    apply (in_cons (w, s) c l) in contra. apply H9 in H10.
+    apply H10 in contra. exact contra.
+    apply NoDup_cons_iff in H8. destruct H8. exact H10.
+    discriminate.
+    intros; destruct (cachelet_invalidation C (w, s)).
+    discriminate.
+    discriminate.
+    discriminate.
+    intros; destruct (NatMap.find s R).
+    discriminate.
+    discriminate.
+  }
+Qed.
+
+Lemma hard : forall r l F V C R F' V' C' R' e ranV ranV',
+  clear_remapping_list r l F V C R = Some (single_level_cache F' V' C' R') ->
+  NatMap.find r V = Some l ->
+  NatMap.find e V = Some ranV ->
+  NatMap.find e V' = Some ranV' ->
+  (forall e' l', NatMap.find e' V = Some l' -> ((forall c, In c l' -> ~ In c F) /\ (forall c, In c F -> ~ In c l'))
+  /\ NoDup(F) /\ NoDup(l') /\ disjoint_VPT(V)) ->
+  (forall e' l', NatMap.find e' V' = Some l' -> ((forall c, In c l' -> ~ In c F') /\ (forall c, In c F' -> ~ In c l'))
+  /\ NoDup(F') /\ NoDup(l') /\ disjoint_VPT(V')).
+Proof.
+  intros r l.
+  induction l.
+  {
+    intros.
+    unfold clear_remapping_list in H.
+    injection H; intros; subst.
+    case_eq (eqb e r); intros V0.
+    {
+      apply cmp_to_eq in V0; subst.
+      assert (NatMap.find r (NatMap.remove r V) = None).
+      apply NatMapFacts.remove_eq_o; reflexivity.
+      rewrite -> H2 in H5. discriminate.
+    }
+    {
+      apply cmp_to_uneq in V0.
+      assert (NatMap.find e (NatMap.remove r V) = NatMap.find e V).
+      apply NatMapFacts.remove_neq_o; apply not_eq_sym; exact V0.
+      rewrite -> H2 in H5; rewrite -> H1 in H5.
+      injection H5; intros; subst.
+      specialize (H3
+
+(* TODO *)
+
+      split; destruct H4. exact H4.
+      split; destruct H7. exact H7.
+      split; destruct H8. exact H8.
+      apply disjoint_VPT_remove; exact H9.
+    }
+  }
+
+Lemma wf3_mlc_dealloc : forall lambda h_tree state k k' index psi psi' F V C R F' V' C' R' enc ranV ranV',
   well_defined_cache_tree h_tree ->
   mlc_deallocation state k lambda h_tree = Some k' ->
   NatMap.find index k = Some psi ->
   NatMap.find index k' = Some psi' ->
   psi = single_level_cache F V C R ->
   psi' = single_level_cache F' V' C' R' ->
-  V_range V enc = Some ranV ->
-  V_range V' enc = Some ranV' ->
-  ((In c ranV -> ~In c F) /\ (In c F -> ~In c ranV)) ->
-  ((In c ranV' -> ~In c F') /\ (In c F' -> ~In c ranV')).
+  NatMap.find (elt:=remapping_list) enc V = Some ranV ->
+  NatMap.find (elt:=remapping_list) enc V' = Some ranV' ->
+  (forall e l, NatMap.find e V = Some l -> ((forall c, In c ranV -> ~In c F) /\ (forall c, In c F -> ~In c ranV)) /\ NoDup(F) /\ NoDup(ranV) /\ disjoint_VPT(V)) ->
+  ((forall c, In c ranV' -> ~In c F') /\ (forall c, In c F' -> ~In c ranV')) /\ NoDup(F') /\ NoDup(ranV') /\ disjoint_VPT(V').
 Proof.
   unfold mlc_deallocation.
   intros lambda h_tree state.
@@ -548,7 +763,7 @@ Proof.
   induction l.
   {
     intros lambda IHTREE k k' index psi psi' F V C R
-    F' V' C' R' c enc ranV ranV' WFH; intros.
+    F' V' C' R' enc ranV ranV' WFH; intros.
     destruct state; destruct e.
     unfold recursive_mlc_deallocation in H.
     injection H; intros; subst k'.
@@ -556,12 +771,12 @@ Proof.
     injection H1; intros; subst psi psi'.
     injection H7; intros; subst F' V' C' R'.
     rewrite -> H5 in H4; injection H4; intros; subst.
-    exact H6.
+    apply (H6 enc ranV). exact H5.
     discriminate.
   }
   {
     intros lambda IHTREE k k' index psi psi' F V C R
-    F' V' C' R' c enc ranV ranV' WFH; intros.
+    F' V' C' R' enc ranV ranV' WFH; intros.
     destruct state; destruct e.
     unfold recursive_mlc_deallocation in H.
     fold recursive_mlc_deallocation in H.
@@ -579,11 +794,11 @@ Proof.
       rewrite -> H7 in H0.
       injection H0; intros; subst s.
       destruct s1.
-      case_eq (V_range v enc). intros.
+      case_eq (NatMap.find enc v). intros.
       destruct l.
       {
-        apply (IHl root_node WFH1 (NatMap.add index (single_level_cache c0 v w s) k) k' index
-        (single_level_cache c0 v w s) psi' c0 v w s F' V' C' R' c enc l0 ranV').
+        apply (IHl root_node WFH1 (NatMap.add index (single_level_cache c v w s) k) k' index
+        (single_level_cache c v w s) psi' c v w s F' V' C' R' enc r0 ranV').
         exact WFH.
         unfold mlc_deallocation. exact H.
         apply NatMapFacts.add_eq_o. reflexivity.
@@ -593,12 +808,42 @@ Proof.
         exact H9.
         exact H5.
         unfold cachelet_deallocation in H8. destruct psi.
+
+
+
+
         case_eq (NatMap.find r v0). intros.
         assert (A0 := H10). destruct (NatMap.find r v0) in A0, H8.
-        injection A0; injection H2; intros; subst c1 v0 w0 s0 r1; clear A0.
-        (* apply (wf3_clear_remapping_list r r1 (single_level_cache c1 v0 w0 s0) (single_level_cache c0 v w s)
-        c1 v0 w0 s0 c0 v w s c) in H8. *)
-        give_up.
+        injection A0; injection H2; intros; subst c0 v0 w0 s0 r1; clear A0.
+        case_eq (eqb r enc); intros.
+        apply cmp_to_eq in H11; subst enc.
+        apply (wf3_clear_remapping_list r r2 F V C R c v w s r0) in H8.
+        exact H8. exact H10. exact H9.
+        rewrite -> H4 in H10.
+        injection H10; intros; subst.
+        exact H6.
+        apply cmp_to_uneq in H11.
+        apply (wf3_clear_remapping_list_uneq r r2 F V C R c v w s enc ranV r0).
+        apply not_eq_sym; exact H11. exact H8. exact H10.
+        exact H4. exact H9. exact H6.
+        destruct H6. destruct H12.
+
+
+        assert (H12 := H8).
+        apply (clear_remapping_list_ranV r r2 F V C R c v w s enc ranV r0) in H8.
+        subst r0.
+        destruct H6; destruct H6; destruct H8.
+        split; split.
+        intros. intros contra.
+        apply H6 in H15.
+        assert (In c0 F -> In c0 c).
+        apply (clear_remapping_list_f r r2 F V C R c v w s c0) in H12.
+        intros; exact H12. exact H10.
+        
+
+
+
+
         discriminate.
         intros; destruct (NatMap.find r v0).
         discriminate.
@@ -706,6 +951,9 @@ Proof.
   intros; injection H1; intros.
   inversion H0. inversion H19; subst.
   - case_eq (NatMap.find lambda m); intros; subst.
+
+
+
     destruct s.
     case_eq (V_range v e); intros.
     assert (V_range v e = Some l1 -> (In c l1 -> ~ In c c0) /\ (In c c0 -> ~In c l1)).
